wip: exp_precomp

code/bignum/Hacl.Spec.Bignum.Exponentiation.fst
@@ -4,24 +4,23 @@ open FStar.Mul
 
 open Lib.IntTypes
 open Lib.Sequence
-open Lib.LoopCombinators
 
 open Hacl.Spec.Bignum.Definitions
-open Hacl.Spec.Bignum
-open Hacl.Spec.Bignum.Montgomery
-open Hacl.Spec.Bignum.ModInvLimb
 
-module BL = Hacl.Spec.Exponentiation.Lemmas
+module Loops = Lib.LoopCombinators
+module E = Hacl.Spec.Exponentiation.Lemmas
 module M = Hacl.Spec.Montgomery.Lemmas
-
+module BN = Hacl.Spec.Bignum
+module BM = Hacl.Spec.Bignum.Montgomery
+module BI = Hacl.Spec.Bignum.ModInvLimb
 
 #reset-options "--z3rlimit 50 --fuel 0 --ifuel 0"
 
 let bn_check_mod_exp #t #nLen n a bBits b =
   let pbits = bits t in
-  let m0 = bn_check_modulus n in
-  let m1 = bn_is_zero_mask b in
-  bn_is_zero_mask_lemma b;
+  let m0 = BM.bn_check_modulus n in
+  let m1 = BN.bn_is_zero_mask b in
+  BN.bn_is_zero_mask_lemma b;
   assert (if v m1 = 0 then bn_v b > 0 else bn_v b = 0);
   assert (v m1 = 0 \/ v m1 = ones_v t);
   let m1' = lognot m1 in
@@ -31,15 +30,15 @@ let bn_check_mod_exp #t #nLen n a bBits b =
   bn_eval_bound b (blocks bBits pbits);
   let m2 =
     if bBits < pbits * blocks bBits pbits then begin
-      bn_lt_pow2_mask_lemma b bBits;
-      bn_lt_pow2_mask b bBits end
+      BN.bn_lt_pow2_mask_lemma b bBits;
+      BN.bn_lt_pow2_mask b bBits end
     else begin
       Math.Lemmas.pow2_le_compat bBits (pbits * blocks bBits pbits);
       ones t SEC end in
   assert (if v m2 = 0 then pow2 bBits <= bn_v b else bn_v b < pow2 bBits);
 
-  let m3 = bn_lt_mask a n in
-  bn_lt_mask_lemma a n;
+  let m3 = BN.bn_lt_mask a n in
+  BN.bn_lt_mask_lemma a n;
   assert (if v m3 = 0 then bn_v a >= bn_v n else bn_v a < bn_v n);
 
   let m = m1' &. m2 &. m3 in
@@ -65,9 +64,9 @@ val bn_mod_exp_f:
   tuple2 (lbignum t nLen) (lbignum t nLen)
 
 let bn_mod_exp_f #t #nLen n mu bBits bLen b i (aM, accM) =
-  let is_bit_set = not (Hacl.Spec.Bignum.Base.unsafe_bool_of_limb0 (bn_get_ith_bit b i)) in
-  let accM = if is_bit_set then bn_mont_mul n mu aM accM else accM in // acc = (acc * a) % n
-  let aM = bn_mont_sqr n mu aM in // a = (a * a) % n
+  let is_bit_set = not (Hacl.Spec.Bignum.Base.unsafe_bool_of_limb0 (BN.bn_get_ith_bit b i)) in
+  let accM = if is_bit_set then BM.bn_mont_mul n mu aM accM else accM in // acc = (acc * a) % n
+  let aM = BM.bn_mont_sqr n mu aM in // a = (a * a) % n
   (aM, accM)
 
 
@@ -84,16 +83,16 @@ val bn_mod_exp_mont:
 
 let bn_mod_exp_mont #t nLen n a acc bBits b r2 =
   let bLen = blocks bBits (bits t) in
-  let mu = mod_inv_limb n.[0] in
+  let mu = BI.mod_inv_limb n.[0] in
 
-  let aM = bn_to_mont n mu r2 a in
-  let accM = bn_to_mont n mu r2 acc in
-  let (aM, accM) = repeati bBits (bn_mod_exp_f n mu bBits bLen b) (aM, accM) in
-  bn_from_mont n mu accM
+  let aM = BM.bn_to_mont n mu r2 a in
+  let accM = BM.bn_to_mont n mu r2 acc in
+  let (aM, accM) = Loops.repeati bBits (bn_mod_exp_f n mu bBits bLen b) (aM, accM) in
+  BM.bn_from_mont n mu accM
 
 
 let bn_mod_exp_precompr2 #t nLen n a bBits b r2 =
-  let acc = bn_from_uint nLen (uint #t 1) in
+  let acc = BN.bn_from_uint nLen (uint #t 1) in
   bn_mod_exp_mont nLen n a acc bBits b r2
 
 
@@ -106,27 +105,25 @@ val bn_mod_exp_f_lemma:
   -> bLen:size_nat{bLen == blocks bBits (bits t)}
   -> b:lbignum t bLen
   -> i:nat{i < bBits}
-  -> aM_accM0: tuple2 (lbignum t nLen) (lbignum t nLen) -> Lemma
+  -> aM0:lbignum t nLen
+  -> accM0:lbignum t nLen -> Lemma
   (requires
-   (let (aM0, accM0) = aM_accM0 in
-    (1 + (bn_v n % pow2 (bits t)) * v mu) % pow2 (bits t) == 0 /\
-    bn_v n % 2 = 1 /\ 1 < bn_v n /\
+    BM.bn_mont_pre n mu /\
     0 < bn_v b /\ bn_v b < pow2 bBits /\
-    bn_v aM0 < bn_v n /\ bn_v accM0 < bn_v n))
+    bn_v aM0 < bn_v n /\ bn_v accM0 < bn_v n)
   (ensures
-   (let (aM0, accM0) = aM_accM0 in
-    let (aM1, accM1) = bn_mod_exp_f n mu bBits bLen b i aM_accM0 in
-    let (aM2, accM2) = BL.mod_exp_mont_f_ll (bits t) nLen (bn_v n) (v mu) bBits (bn_v b) i (bn_v aM0, bn_v accM0) in
+   (let (aM1, accM1) = bn_mod_exp_f n mu bBits bLen b i (aM0, accM0) in
+    let (aM2, accM2) = E.mod_exp_mont_f_ll (bits t) nLen (bn_v n) (v mu) bBits (bn_v b) i (bn_v aM0, bn_v accM0) in
     bn_v aM1 == aM2 /\ bn_v accM1 == accM2 /\
     bn_v aM1 < bn_v n /\ bn_v accM1 < bn_v n))
 
-let bn_mod_exp_f_lemma #t #nLen n mu bBits bLen b i (aM0, accM0) =
+let bn_mod_exp_f_lemma #t #nLen n mu bBits bLen b i aM0 accM0 =
   let (aM1, accM1) = bn_mod_exp_f n mu bBits bLen b i (aM0, accM0) in
-  let (aM2, accM2) = BL.mod_exp_mont_f_ll (bits t) nLen (bn_v n) (v mu) bBits (bn_v b) i (bn_v aM0, bn_v accM0) in
-  bn_mont_sqr_lemma n mu aM0;
+  let (aM2, accM2) = E.mod_exp_mont_f_ll (bits t) nLen (bn_v n) (v mu) bBits (bn_v b) i (bn_v aM0, bn_v accM0) in
+  BM.bn_mont_sqr_lemma n mu aM0;
   assert (bn_v aM1 == aM2);
-  bn_get_ith_bit_lemma b i;
-  if (bn_v b / pow2 i % 2 = 1) then bn_mont_mul_lemma n mu aM0 accM0;
+  BN.bn_get_ith_bit_lemma b i;
+  if (bn_v b / pow2 i % 2 = 1) then BM.bn_mont_mul_lemma n mu aM0 accM0;
   assert (bn_v accM1 == accM2)
 
 
@@ -139,38 +136,36 @@ val bn_mod_exp_mont_loop_lemma:
   -> bLen:size_nat{bLen == blocks bBits (bits t)}
   -> b:lbignum t bLen
   -> i:size_nat{i <= bBits}
-  -> aM_accM0: tuple2 (lbignum t nLen) (lbignum t nLen) -> Lemma
+  -> aM0:lbignum t nLen
+  -> accM0:lbignum t nLen -> Lemma
   (requires
-   (let (aM0, accM0) = aM_accM0 in
-    (1 + (bn_v n % pow2 (bits t)) * v mu) % pow2 (bits t) == 0 /\
-    bn_v n % 2 = 1 /\ 1 < bn_v n /\
+    BM.bn_mont_pre n mu /\
     0 < bn_v b /\ bn_v b < pow2 bBits /\
-    bn_v aM0 < bn_v n /\ bn_v accM0 < bn_v n))
+    bn_v aM0 < bn_v n /\ bn_v accM0 < bn_v n)
   (ensures
-   (let (aM0, accM0) = aM_accM0 in
-    let (aM1, accM1) = repeati i (bn_mod_exp_f n mu bBits bLen b) (aM0, accM0) in
-    let (aM2, accM2) = repeati i (BL.mod_exp_mont_f_ll (bits t) nLen (bn_v n) (v mu) bBits (bn_v b)) (bn_v aM0, bn_v accM0) in
+   (let (aM1, accM1) = Loops.repeati i (bn_mod_exp_f n mu bBits bLen b) (aM0, accM0) in
+    let (aM2, accM2) = Loops.repeati i (E.mod_exp_mont_f_ll (bits t) nLen (bn_v n) (v mu) bBits (bn_v b)) (bn_v aM0, bn_v accM0) in
     bn_v aM1 == aM2 /\ bn_v accM1 == accM2 /\
     bn_v aM1 < bn_v n /\ bn_v accM1 < bn_v n))
 
-let rec bn_mod_exp_mont_loop_lemma #t #nLen n mu bBits bLen b i (aM0, accM0) =
-  let (aM1, accM1) = repeati i (bn_mod_exp_f n mu bBits bLen b) (aM0, accM0) in
-  let (aM2, accM2) = repeati i (BL.mod_exp_mont_f_ll (bits t) nLen (bn_v n) (v mu) bBits (bn_v b)) (bn_v aM0, bn_v accM0) in
+let rec bn_mod_exp_mont_loop_lemma #t #nLen n mu bBits bLen b i aM0 accM0 =
+  let (aM1, accM1) = Loops.repeati i (bn_mod_exp_f n mu bBits bLen b) (aM0, accM0) in
+  let (aM2, accM2) = Loops.repeati i (E.mod_exp_mont_f_ll (bits t) nLen (bn_v n) (v mu) bBits (bn_v b)) (bn_v aM0, bn_v accM0) in
 
   if i = 0 then begin
-    eq_repeati0 i (bn_mod_exp_f n mu bBits bLen b) (aM0, accM0);
-    eq_repeati0 i (BL.mod_exp_mont_f_ll (bits t) nLen (bn_v n) (v mu) bBits (bn_v b)) (bn_v aM0, bn_v accM0);
+    Loops.eq_repeati0 i (bn_mod_exp_f n mu bBits bLen b) (aM0, accM0);
+    Loops.eq_repeati0 i (E.mod_exp_mont_f_ll (bits t) nLen (bn_v n) (v mu) bBits (bn_v b)) (bn_v aM0, bn_v accM0);
     () end
   else begin
-    unfold_repeati i (bn_mod_exp_f n mu bBits bLen b) (aM0, accM0) (i - 1);
-    unfold_repeati i (BL.mod_exp_mont_f_ll (bits t) nLen (bn_v n) (v mu) bBits (bn_v b)) (bn_v aM0, bn_v accM0) (i - 1);
-    let (aM3, accM3) = repeati (i - 1) (bn_mod_exp_f n mu bBits bLen b) (aM0, accM0) in
-    let (aM4, accM4) = repeati (i - 1) (BL.mod_exp_mont_f_ll (bits t) nLen (bn_v n) (v mu) bBits (bn_v b)) (bn_v aM0, bn_v accM0) in
+    Loops.unfold_repeati i (bn_mod_exp_f n mu bBits bLen b) (aM0, accM0) (i - 1);
+    Loops.unfold_repeati i (E.mod_exp_mont_f_ll (bits t) nLen (bn_v n) (v mu) bBits (bn_v b)) (bn_v aM0, bn_v accM0) (i - 1);
+    let (aM3, accM3) = Loops.repeati (i - 1) (bn_mod_exp_f n mu bBits bLen b) (aM0, accM0) in
+    let (aM4, accM4) = Loops.repeati (i - 1) (E.mod_exp_mont_f_ll (bits t) nLen (bn_v n) (v mu) bBits (bn_v b)) (bn_v aM0, bn_v accM0) in
     assert ((aM1, accM1) == bn_mod_exp_f n mu bBits bLen b (i - 1) (aM3, accM3));
-    assert ((aM2, accM2) == BL.mod_exp_mont_f_ll (bits t) nLen (bn_v n) (v mu) bBits (bn_v b) (i - 1) (aM4, accM4));
-    bn_mod_exp_mont_loop_lemma n mu bBits bLen b (i - 1) (aM0, accM0);
+    assert ((aM2, accM2) == E.mod_exp_mont_f_ll (bits t) nLen (bn_v n) (v mu) bBits (bn_v b) (i - 1) (aM4, accM4));
+    bn_mod_exp_mont_loop_lemma n mu bBits bLen b (i - 1) aM0 accM0;
     assert (bn_v aM3 == aM4 /\ bn_v accM3 == accM4);
-    bn_mod_exp_f_lemma n mu bBits bLen b (i - 1) (aM3, accM3);
+    bn_mod_exp_f_lemma n mu bBits bLen b (i - 1) aM3 accM3;
     () end
 
 
@@ -187,42 +182,42 @@ val bn_mod_exp_mont_lemma_aux:
     0 < bn_v b /\ bn_v b < pow2 bBits /\ bn_v a < bn_v n /\
     bn_v r2 == pow2 (2 * bits t * nLen) % bn_v n)
   (ensures
-   (let mu = mod_inv_limb n.[0] in
+   (let mu = BI.mod_inv_limb n.[0] in
     let res1 = bn_mod_exp_precompr2 nLen n a bBits b r2 in
-    let res2 = BL.mod_exp_mont_ll (bits t) nLen (bn_v n) (v mu) (bn_v a) bBits (bn_v b) in
+    let res2 = E.mod_exp_mont_ll (bits t) nLen (bn_v n) (v mu) (bn_v a) bBits (bn_v b) in
     bn_v res1 == res2 /\ bn_v res1 < bn_v n))
 
 let bn_mod_exp_mont_lemma_aux #t nLen n a bBits b r2 =
   let bLen = blocks bBits (bits t) in
 
-  let acc = bn_from_uint nLen (uint #t 1) in
-  bn_from_uint_lemma nLen (uint #t 1);
+  let acc = BN.bn_from_uint nLen (uint #t 1) in
+  BN.bn_from_uint_lemma nLen (uint #t 1);
   assert (bn_v acc == 1);
 
-  let mu = mod_inv_limb n.[0] in
+  let mu = BI.mod_inv_limb n.[0] in
   bn_eval_index n 0;
   assert (bn_v n % pow2 (bits t) == v n.[0]);
   Math.Lemmas.pow2_modulo_modulo_lemma_1 (bn_v n) 2 (bits t);
   assert (v n.[0] % 2 = 1); // since bn_v n % 2 = 1
-  mod_inv_limb_lemma n.[0];
+  BI.mod_inv_limb_lemma n.[0];
 
-  let aM0 = bn_to_mont n mu r2 a in
-  bn_to_mont_lemma n mu r2 a;
+  let aM0 = BM.bn_to_mont n mu r2 a in
+  BM.bn_to_mont_lemma n mu r2 a;
 
-  let accM0 = bn_to_mont n mu r2 acc in
-  bn_to_mont_lemma n mu r2 acc;
+  let accM0 = BM.bn_to_mont n mu r2 acc in
+  BM.bn_to_mont_lemma n mu r2 acc;
 
-  let (aM1, accM1) = repeati bBits (bn_mod_exp_f n mu bBits bLen b) (aM0, accM0) in
-  bn_mod_exp_mont_loop_lemma n mu bBits bLen b bBits (aM0, accM0);
+  let (aM1, accM1) = Loops.repeati bBits (bn_mod_exp_f n mu bBits bLen b) (aM0, accM0) in
+  bn_mod_exp_mont_loop_lemma n mu bBits bLen b bBits aM0 accM0;
 
-  let res = bn_from_mont n mu accM1 in
-  bn_from_mont_lemma n mu accM1
+  let res = BM.bn_from_mont n mu accM1 in
+  BM.bn_from_mont_lemma n mu accM1
 
 
 let bn_mod_exp_precompr2_lemma #t nLen n a bBits b r2 =
-  let mu = mod_inv_limb n.[0] in
+  let mu = BI.mod_inv_limb n.[0] in
   let res1 = bn_mod_exp_precompr2 nLen n a bBits b r2 in
-  let res2 = BL.mod_exp_mont_ll (bits t) nLen (bn_v n) (v mu) (bn_v a) bBits (bn_v b) in
+  let res2 = E.mod_exp_mont_ll (bits t) nLen (bn_v n) (v mu) (bn_v a) bBits (bn_v b) in
   bn_mod_exp_mont_lemma_aux nLen n a bBits b r2;
   assert (bn_v res1 == res2 /\ bn_v res1 < bn_v n);
 
@@ -230,13 +225,12 @@ let bn_mod_exp_precompr2_lemma #t nLen n a bBits b r2 =
   assert (bn_v n % pow2 (bits t) == v n.[0]);
   Math.Lemmas.pow2_modulo_modulo_lemma_1 (bn_v n) 2 (bits t);
   assert (v n.[0] % 2 = 1); // since bn_v n % 2 = 1
-  mod_inv_limb_lemma n.[0];
+  BI.mod_inv_limb_lemma n.[0];
   assert ((1 + (bn_v n % pow2 (bits t)) * v mu) % pow2 (bits t) == 0);
 
   bn_eval_bound n nLen;
-  let d, k = M.eea_pow2_odd (bits t * nLen) (bn_v n) in
   M.mont_preconditions (bits t) nLen (bn_v n) (v mu);
-  BL.mod_exp_mont_ll_lemma (bits t) nLen (bn_v n) d (v mu) (bn_v a) bBits (bn_v b)
+  E.mod_exp_mont_ll_lemma (bits t) nLen (bn_v n) (v mu) (bn_v a) bBits (bn_v b)
 
 ///
 ///  Montgomery ladder for exponentiation
@@ -258,11 +252,11 @@ val bn_mod_exp_mont_ladder_f:
   tuple3 (lbignum t nLen) (lbignum t nLen) (limb t)
 
 let bn_mod_exp_mont_ladder_f #t #nLen n mu bBits bLen b i (rM0, rM1, privbit) =
-  let bit = bn_get_ith_bit b (bBits - i - 1) in
+  let bit = BN.bn_get_ith_bit b (bBits - i - 1) in
   let sw = bit ^. privbit in
-  let rM0, rM1 = cswap2 sw rM0 rM1 in
-  let rM0' = bn_mont_sqr n mu rM0 in // rM0 * rM0 % n
-  let rM1' = bn_mont_mul n mu rM1 rM0 in // rM1 * rM0 % n
+  let rM0, rM1 = BN.cswap2 sw rM0 rM1 in
+  let rM0' = BM.bn_mont_sqr n mu rM0 in // rM0 * rM0 % n
+  let rM1' = BM.bn_mont_mul n mu rM1 rM0 in // rM1 * rM0 % n
   (rM0', rM1', bit)
 
 
@@ -279,19 +273,19 @@ val bn_mod_exp_mont_ladder_:
 
 let bn_mod_exp_mont_ladder_ #t nLen n a one bBits b r2 =
   let bLen = blocks bBits (bits t) in
-  let mu = mod_inv_limb n.[0] in
+  let mu = BI.mod_inv_limb n.[0] in
 
-  let rM0 = bn_to_mont n mu r2 one in
-  let rM1 = bn_to_mont n mu r2 a in
+  let rM0 = BM.bn_to_mont n mu r2 one in
+  let rM1 = BM.bn_to_mont n mu r2 a in
   let sw = uint #t 0 in
-  let (rM0', rM1', sw') = repeat_gen bBits (bn_mod_exp_mont_ladder_t t nLen bBits)
+  let (rM0', rM1', sw') = Loops.repeat_gen bBits (bn_mod_exp_mont_ladder_t t nLen bBits)
     (bn_mod_exp_mont_ladder_f n mu bBits bLen b) (rM0, rM1, sw) in
-  let (rM0', rM1') = cswap2 sw' rM0' rM1' in
-  bn_from_mont n mu rM0'
+  let (rM0', rM1') = BN.cswap2 sw' rM0' rM1' in
+  BM.bn_from_mont n mu rM0'
 
 
 let bn_mod_exp_mont_ladder_precompr2 #t nLen n a bBits b r2 =
-  let acc = bn_from_uint nLen (uint #t 1) in
+  let acc = BN.bn_from_uint nLen (uint #t 1) in
   bn_mod_exp_mont_ladder_ nLen n a acc bBits b r2
 
 
@@ -324,34 +318,35 @@ val bn_mod_exp_mont_ladder_f_lemma:
   -> bLen:size_nat{bLen == blocks bBits (bits t)}
   -> b:lbignum t bLen
   -> i:nat{i < bBits}
-  -> rM0_rM1_sw: tuple3 (lbignum t nLen) (lbignum t nLen) (limb t) -> Lemma
+  -> rM0:lbignum t nLen
+  -> rM1:lbignum t nLen
+  -> sw:limb t -> Lemma
   (requires
-   (let (rM0, rM1, sw) = rM0_rM1_sw in
-    (1 + (bn_v n % pow2 (bits t)) * v mu) % pow2 (bits t) == 0 /\
-    bn_v n % 2 = 1 /\ 1 < bn_v n /\
+    BM.bn_mont_pre n mu /\
     0 < bn_v b /\ bn_v b < pow2 bBits /\
-    bn_v rM0 < bn_v n /\ bn_v rM1 < bn_v n /\ v sw <= 1))
+    bn_v rM0 < bn_v n /\ bn_v rM1 < bn_v n /\ v sw <= 1)
   (ensures
-   (let (rM0, rM1, sw) = rM0_rM1_sw in
-    let (rM0', rM1', sw') = bn_mod_exp_mont_ladder_f n mu bBits bLen b i (rM0, rM1, sw) in
-    let (rM0'', rM1'', sw'') = BL.mod_exp_mont_ladder_swap_f_ll (bits t) nLen (bn_v n) (v mu) bBits (bn_v b) i (bn_v rM0, bn_v rM1, v sw) in
+   (let (rM0', rM1', sw') = bn_mod_exp_mont_ladder_f n mu bBits bLen b i (rM0, rM1, sw) in
+    let (rM0'', rM1'', sw'') = E.mod_exp_mont_ladder_swap_f_ll
+      (bits t) nLen (bn_v n) (v mu) bBits (bn_v b) i (bn_v rM0, bn_v rM1, v sw) in
     bn_v rM0' == rM0'' /\ bn_v rM1' == rM1'' /\ v sw' == sw'' /\
     bn_v rM0' < bn_v n /\ bn_v rM1' < bn_v n /\ v sw' <= 1))
 
-let bn_mod_exp_mont_ladder_f_lemma #t #nLen n mu bBits bLen b i (rM0, rM1, sw) =
+let bn_mod_exp_mont_ladder_f_lemma #t #nLen n mu bBits bLen b i rM0 rM1 sw =
   let (rM0', rM1', sw') = bn_mod_exp_mont_ladder_f n mu bBits bLen b i (rM0, rM1, sw) in
-  let (rM0'', rM1'', sw'') = BL.mod_exp_mont_ladder_swap_f_ll (bits t) nLen (bn_v n) (v mu) bBits (bn_v b) i (bn_v rM0, bn_v rM1, v sw) in
-  let bit = bn_get_ith_bit b (bBits - i - 1) in
-  bn_get_ith_bit_lemma b (bBits - i - 1);
+  let (rM0'', rM1'', sw'') = E.mod_exp_mont_ladder_swap_f_ll
+    (bits t) nLen (bn_v n) (v mu) bBits (bn_v b) i (bn_v rM0, bn_v rM1, v sw) in
+  let bit = BN.bn_get_ith_bit b (bBits - i - 1) in
+  BN.bn_get_ith_bit_lemma b (bBits - i - 1);
   //assert (v bit == bn_v b / pow2 (bBits - i - 1) % 2);
   let sw1 = bit ^. sw in
   lemma_bit_xor_is_sum_mod2 bit sw;
-  let rM2, rM3 = cswap2 sw1 rM0 rM1 in
-  cswap2_lemma sw1 rM0 rM1;
-  let rM2' = bn_mont_sqr n mu rM2 in
-  bn_mont_sqr_lemma n mu rM2;
-  let rM3' = bn_mont_mul n mu rM3 rM2 in
-  bn_mont_mul_lemma n mu rM3 rM2;
+  let rM2, rM3 = BN.cswap2 sw1 rM0 rM1 in
+  BN.cswap2_lemma sw1 rM0 rM1;
+  let rM2' = BM.bn_mont_sqr n mu rM2 in
+  BM.bn_mont_sqr_lemma n mu rM2;
+  let rM3' = BM.bn_mont_mul n mu rM3 rM2 in
+  BM.bn_mont_mul_lemma n mu rM3 rM2;
   assert (rM0' == rM2' /\ rM1' == rM3' /\ sw' == bit);
   assert (bn_v rM0' == rM0'' /\ bn_v rM1' == rM1'' /\ v sw' == sw'')
 
@@ -365,44 +360,43 @@ val bn_mod_exp_mont_ladder_loop_lemma:
   -> bLen:size_nat{bLen == blocks bBits (bits t)}
   -> b:lbignum t bLen
   -> i:size_nat{i <= bBits}
-  -> rM0_rM1_sw: tuple3 (lbignum t nLen) (lbignum t nLen) (limb t) -> Lemma
+  -> rM0:lbignum t nLen
+  -> rM1:lbignum t nLen
+  -> sw:limb t -> Lemma
   (requires
-   (let (rM0, rM1, sw) = rM0_rM1_sw in
-    (1 + (bn_v n % pow2 (bits t)) * v mu) % pow2 (bits t) == 0 /\
-    bn_v n % 2 = 1 /\ 1 < bn_v n /\
+    BM.bn_mont_pre n mu /\
     0 < bn_v b /\ bn_v b < pow2 bBits /\
-    bn_v rM0 < bn_v n /\ bn_v rM1 < bn_v n /\ v sw <= 1))
+    bn_v rM0 < bn_v n /\ bn_v rM1 < bn_v n /\ v sw <= 1)
   (ensures
-   (let (rM0, rM1, sw) = rM0_rM1_sw in
-    let (rM0', rM1', sw') = repeat_gen i (bn_mod_exp_mont_ladder_t t nLen bBits)
+   (let (rM0', rM1', sw') = Loops.repeat_gen i (bn_mod_exp_mont_ladder_t t nLen bBits)
       (bn_mod_exp_mont_ladder_f n mu bBits bLen b) (rM0, rM1, sw) in
-    let (rM0'', rM1'', sw'') = repeati i
-      (BL.mod_exp_mont_ladder_swap_f_ll (bits t) nLen (bn_v n) (v mu) bBits (bn_v b)) (bn_v rM0, bn_v rM1, v sw) in
+    let (rM0'', rM1'', sw'') = Loops.repeati i
+      (E.mod_exp_mont_ladder_swap_f_ll (bits t) nLen (bn_v n) (v mu) bBits (bn_v b)) (bn_v rM0, bn_v rM1, v sw) in
     bn_v rM0' == rM0'' /\ bn_v rM1' == rM1'' /\ v sw' == sw'' /\
     bn_v rM0' < bn_v n /\ bn_v rM1' < bn_v n /\ v sw' <= 1))
 
-let rec bn_mod_exp_mont_ladder_loop_lemma #t #nLen n mu bBits bLen b i (rM0, rM1, sw) =
-  let (rM0', rM1', sw') = repeat_gen i (bn_mod_exp_mont_ladder_t t nLen bBits)
+let rec bn_mod_exp_mont_ladder_loop_lemma #t #nLen n mu bBits bLen b i rM0 rM1 sw =
+  let (rM0', rM1', sw') = Loops.repeat_gen i (bn_mod_exp_mont_ladder_t t nLen bBits)
       (bn_mod_exp_mont_ladder_f n mu bBits bLen b) (rM0, rM1, sw) in
-  let (rM0'', rM1'', sw'') = repeati i
-    (BL.mod_exp_mont_ladder_swap_f_ll (bits t) nLen (bn_v n) (v mu) bBits (bn_v b)) (bn_v rM0, bn_v rM1, v sw) in
+  let (rM0'', rM1'', sw'') = Loops.repeati i
+    (E.mod_exp_mont_ladder_swap_f_ll (bits t) nLen (bn_v n) (v mu) bBits (bn_v b)) (bn_v rM0, bn_v rM1, v sw) in
 
   if i = 0 then begin
-    eq_repeat_gen0 i (bn_mod_exp_mont_ladder_t t nLen bBits) (bn_mod_exp_mont_ladder_f n mu bBits bLen b) (rM0, rM1, sw);
-    eq_repeati0 i (BL.mod_exp_mont_ladder_swap_f_ll (bits t) nLen (bn_v n) (v mu) bBits (bn_v b)) (bn_v rM0, bn_v rM1, v sw);
+    Loops.eq_repeat_gen0 i (bn_mod_exp_mont_ladder_t t nLen bBits) (bn_mod_exp_mont_ladder_f n mu bBits bLen b) (rM0, rM1, sw);
+    Loops.eq_repeati0 i (E.mod_exp_mont_ladder_swap_f_ll (bits t) nLen (bn_v n) (v mu) bBits (bn_v b)) (bn_v rM0, bn_v rM1, v sw);
     () end
   else begin
-    unfold_repeat_gen i (bn_mod_exp_mont_ladder_t t nLen bBits) (bn_mod_exp_mont_ladder_f n mu bBits bLen b) (rM0, rM1, sw) (i - 1);
-    unfold_repeati i (BL.mod_exp_mont_ladder_swap_f_ll (bits t) nLen (bn_v n) (v mu) bBits (bn_v b)) (bn_v rM0, bn_v rM1, v sw) (i - 1);
+    Loops.unfold_repeat_gen i (bn_mod_exp_mont_ladder_t t nLen bBits) (bn_mod_exp_mont_ladder_f n mu bBits bLen b) (rM0, rM1, sw) (i - 1);
+    Loops.unfold_repeati i (E.mod_exp_mont_ladder_swap_f_ll (bits t) nLen (bn_v n) (v mu) bBits (bn_v b)) (bn_v rM0, bn_v rM1, v sw) (i - 1);
 
-    let (rM2', rM3', sw1') = repeat_gen (i - 1) (bn_mod_exp_mont_ladder_t t nLen bBits)
+    let (rM2', rM3', sw1') = Loops.repeat_gen (i - 1) (bn_mod_exp_mont_ladder_t t nLen bBits)
       (bn_mod_exp_mont_ladder_f n mu bBits bLen b) (rM0, rM1, sw) in
-    let (rM2'', rM3'', sw1'') = repeati (i - 1) (BL.mod_exp_mont_ladder_swap_f_ll (bits t) nLen (bn_v n) (v mu) bBits (bn_v b)) (bn_v rM0, bn_v rM1, v sw) in
+    let (rM2'', rM3'', sw1'') = Loops.repeati (i - 1) (E.mod_exp_mont_ladder_swap_f_ll (bits t) nLen (bn_v n) (v mu) bBits (bn_v b)) (bn_v rM0, bn_v rM1, v sw) in
     assert ((rM0', rM1', sw') == bn_mod_exp_mont_ladder_f n mu bBits bLen b (i - 1) (rM2', rM3', sw1'));
-    assert ((rM0'', rM1'', sw'') == BL.mod_exp_mont_ladder_swap_f_ll (bits t) nLen (bn_v n) (v mu) bBits (bn_v b) (i - 1) (rM2'', rM3'', sw1''));
-    bn_mod_exp_mont_ladder_loop_lemma n mu bBits bLen b (i - 1) (rM0, rM1, sw);
+    assert ((rM0'', rM1'', sw'') == E.mod_exp_mont_ladder_swap_f_ll (bits t) nLen (bn_v n) (v mu) bBits (bn_v b) (i - 1) (rM2'', rM3'', sw1''));
+    bn_mod_exp_mont_ladder_loop_lemma n mu bBits bLen b (i - 1) rM0 rM1 sw;
     assert (bn_v rM2' == rM2'' /\ bn_v rM3' == rM3'' /\ v sw1' == sw1'');
-    bn_mod_exp_mont_ladder_f_lemma n mu bBits bLen b (i - 1) (rM2', rM3', sw1');
+    bn_mod_exp_mont_ladder_f_lemma n mu bBits bLen b (i - 1) rM2' rM3' sw1';
     () end
 
 
@@ -419,46 +413,46 @@ val bn_mod_exp_mont_ladder_lemma_aux:
     0 < bn_v b /\ bn_v b < pow2 bBits /\ bn_v a < bn_v n /\
     bn_v r2 == pow2 (2 * bits t * nLen) % bn_v n)
   (ensures
-   (let mu = mod_inv_limb n.[0] in
+   (let mu = BI.mod_inv_limb n.[0] in
     let res1 = bn_mod_exp_mont_ladder_precompr2 nLen n a bBits b r2 in
-    let res2 = BL.mod_exp_mont_ladder_swap_ll (bits t) nLen (bn_v n) (v mu) (bn_v a) bBits (bn_v b) in
+    let res2 = E.mod_exp_mont_ladder_swap_ll (bits t) nLen (bn_v n) (v mu) (bn_v a) bBits (bn_v b) in
     bn_v res1 == res2 /\ bn_v res1 < bn_v n))
 
 let bn_mod_exp_mont_ladder_lemma_aux #t nLen n a bBits b r2 =
   let bLen = blocks bBits (bits t) in
 
-  let one = bn_from_uint nLen (uint #t 1) in
-  bn_from_uint_lemma nLen (uint #t 1);
+  let one = BN.bn_from_uint nLen (uint #t 1) in
+  BN.bn_from_uint_lemma nLen (uint #t 1);
   assert (bn_v one == 1);
 
-  let mu = mod_inv_limb n.[0] in
+  let mu = BI.mod_inv_limb n.[0] in
   bn_eval_index n 0;
   assert (bn_v n % pow2 (bits t) == v n.[0]);
   Math.Lemmas.pow2_modulo_modulo_lemma_1 (bn_v n) 2 (bits t);
   assert (v n.[0] % 2 = 1); // since bn_v n % 2 = 1
-  mod_inv_limb_lemma n.[0];
+  BI.mod_inv_limb_lemma n.[0];
 
-  let rM0 = bn_to_mont n mu r2 one in
-  bn_to_mont_lemma n mu r2 one;
+  let rM0 = BM.bn_to_mont n mu r2 one in
+  BM.bn_to_mont_lemma n mu r2 one;
 
-  let rM1 = bn_to_mont n mu r2 a in
-  bn_to_mont_lemma n mu r2 a;
+  let rM1 = BM.bn_to_mont n mu r2 a in
+  BM.bn_to_mont_lemma n mu r2 a;
 
   let sw = uint #t 0 in
-  let (rM0', rM1', sw') = repeat_gen bBits (bn_mod_exp_mont_ladder_t t nLen bBits)
+  let (rM0', rM1', sw') = Loops.repeat_gen bBits (bn_mod_exp_mont_ladder_t t nLen bBits)
     (bn_mod_exp_mont_ladder_f n mu bBits bLen b) (rM0, rM1, sw) in
-  bn_mod_exp_mont_ladder_loop_lemma n mu bBits bLen b bBits (rM0, rM1, sw);
+  bn_mod_exp_mont_ladder_loop_lemma n mu bBits bLen b bBits rM0 rM1 sw;
 
-  let (rM0'', rM1'') = cswap2 sw' rM0' rM1' in
-  cswap2_lemma sw' rM0' rM1';
-  let res = bn_from_mont n mu rM0'' in
-  bn_from_mont_lemma n mu rM0''
+  let (rM0'', rM1'') = BN.cswap2 sw' rM0' rM1' in
+  BN.cswap2_lemma sw' rM0' rM1';
+  let res = BM.bn_from_mont n mu rM0'' in
+  BM.bn_from_mont_lemma n mu rM0''
 
 
 let bn_mod_exp_mont_ladder_precompr2_lemma #t nLen n a bBits b r2 =
-  let mu = mod_inv_limb n.[0] in
+  let mu = BI.mod_inv_limb n.[0] in
   let res1 = bn_mod_exp_mont_ladder_precompr2 nLen n a bBits b r2 in
-  let res2 = BL.mod_exp_mont_ladder_swap_ll (bits t) nLen (bn_v n) (v mu) (bn_v a) bBits (bn_v b) in
+  let res2 = E.mod_exp_mont_ladder_swap_ll (bits t) nLen (bn_v n) (v mu) (bn_v a) bBits (bn_v b) in
   bn_mod_exp_mont_ladder_lemma_aux nLen n a bBits b r2;
   assert (bn_v res1 == res2 /\ bn_v res1 < bn_v n);
 
@@ -466,32 +460,31 @@ let bn_mod_exp_mont_ladder_precompr2_lemma #t nLen n a bBits b r2 =
   assert (bn_v n % pow2 (bits t) == v n.[0]);
   Math.Lemmas.pow2_modulo_modulo_lemma_1 (bn_v n) 2 (bits t);
   assert (v n.[0] % 2 = 1); // since bn_v n % 2 = 1
-  mod_inv_limb_lemma n.[0];
+  BI.mod_inv_limb_lemma n.[0];
   assert ((1 + (bn_v n % pow2 (bits t)) * v mu) % pow2 (bits t) == 0);
 
   bn_eval_bound n nLen;
-  let d, k = M.eea_pow2_odd (bits t * nLen) (bn_v n) in
   M.mont_preconditions (bits t) nLen (bn_v n) (v mu);
-  BL.mod_exp_mont_ladder_swap_ll_lemma (bits t) nLen (bn_v n) d (v mu) (bn_v a) bBits (bn_v b)
+  E.mod_exp_mont_ladder_swap_ll_lemma (bits t) nLen (bn_v n) (v mu) (bn_v a) bBits (bn_v b)
 
 
 let bn_mod_exp #t nLen nBits n a bBits b =
-  let r2 = bn_precomp_r2_mod_n nBits n in
+  let r2 = BM.bn_precomp_r2_mod_n nBits n in
   bn_mod_exp_precompr2 nLen n a bBits b r2
 
 
 let bn_mod_exp_lemma #t nLen nBits n a bBits b =
-  let r2 = bn_precomp_r2_mod_n nBits n in
-  bn_precomp_r2_mod_n_lemma nBits n;
+  let r2 = BM.bn_precomp_r2_mod_n nBits n in
+  BM.bn_precomp_r2_mod_n_lemma nBits n;
   bn_mod_exp_precompr2_lemma nLen n a bBits b r2
 
 
 let bn_mod_exp_mont_ladder #t nLen nBits n a bBits b =
-  let r2 = bn_precomp_r2_mod_n nBits n in
+  let r2 = BM.bn_precomp_r2_mod_n nBits n in
   bn_mod_exp_mont_ladder_precompr2 nLen n a bBits b r2
 
 
 let bn_mod_exp_mont_ladder_lemma #t nLen nBits n a bBits b =
-  let r2 = bn_precomp_r2_mod_n nBits n in
-  bn_precomp_r2_mod_n_lemma nBits n;
+  let r2 = BM.bn_precomp_r2_mod_n nBits n in
+  BM.bn_precomp_r2_mod_n_lemma nBits n;
   bn_mod_exp_mont_ladder_precompr2_lemma nLen n a bBits b r2
