code/bignum/Hacl.Spec.Bignum.Montgomery.fst
@@ -4,26 +4,26 @@ open FStar.Mul
 
 open Lib.IntTypes
 open Lib.Sequence
-open Lib.LoopCombinators
 
 open Hacl.Spec.Bignum.Base
 open Hacl.Spec.Bignum.Definitions
-open Hacl.Spec.Bignum
 
+module Loops = Lib.LoopCombinators
+module BN = Hacl.Spec.Bignum
 
 #reset-options "--z3rlimit 100 --fuel 0 --ifuel 0"
 
 let bn_check_modulus #t #nLen n =
-  let one = bn_from_uint nLen (uint #t 1) in
-  bn_from_uint_lemma nLen (uint #t 1);
-  let bit0 = bn_is_odd n in
-  bn_is_odd_lemma n;
+  let one = BN.bn_from_uint nLen (uint #t 1) in
+  BN.bn_from_uint_lemma nLen (uint #t 1);
+  let bit0 = BN.bn_is_odd n in
+  BN.bn_is_odd_lemma n;
   assert (v bit0 == bn_v n % 2);
   let m0 = uint #t 0 -. bit0 in
   assert (v m0 == (if bn_v n % 2 = 1 then v (ones t SEC) else v (zeros t SEC)));
 
-  let m1 = bn_lt_mask one n in
-  bn_lt_mask_lemma one n;
+  let m1 = BN.bn_lt_mask one n in
+  BN.bn_lt_mask_lemma one n;
   assert (v m1 == (if 1 < bn_v n then v (ones t SEC) else v (zeros t SEC)));
   let m = m0 &. m1 in
   logand_lemma m0 m1;
@@ -32,25 +32,25 @@ let bn_check_modulus #t #nLen n =
 
 
 val bn_lshift1_mod_n: #t:limb_t -> #len:size_nat -> n:lbignum t len -> i:nat -> b:lbignum t len -> lbignum t len
-let bn_lshift1_mod_n #t #len n i b = bn_add_mod_n n b b
+let bn_lshift1_mod_n #t #len n i b = BN.bn_add_mod_n n b b
 
 val bn_lshift1_mod_n_lemma: #t:limb_t -> #len:size_nat -> n:lbignum t len -> i:nat -> b:lbignum t len -> Lemma
   (requires 0 < bn_v n /\ bn_v b < bn_v n)
   (ensures  bn_v (bn_lshift1_mod_n n i b) == 2 * bn_v b % bn_v n)
 let bn_lshift1_mod_n_lemma #t #len n i b =
-  bn_add_mod_n_lemma n b b
+  BN.bn_add_mod_n_lemma n b b
 
 val bn_mul_by_pow2: #t:limb_t -> len:size_nat -> n:lbignum t len -> b:lbignum t len -> k:nat -> Lemma
   (requires 0 < bn_v n /\ bn_v b < bn_v n)
-  (ensures  bn_v (repeati k (bn_lshift1_mod_n n) b) == pow2 k * bn_v b % bn_v n)
+  (ensures  bn_v (Loops.repeati k (bn_lshift1_mod_n n) b) == pow2 k * bn_v b % bn_v n)
 let rec bn_mul_by_pow2 #t len n b k =
-  if k = 0 then eq_repeati0 k (bn_lshift1_mod_n n) b
+  if k = 0 then Loops.eq_repeati0 k (bn_lshift1_mod_n n) b
   else begin
-    let res = repeati k (bn_lshift1_mod_n n) b in
-    let res0 = repeati (k - 1) (bn_lshift1_mod_n n) b in
+    let res = Loops.repeati k (bn_lshift1_mod_n n) b in
+    let res0 = Loops.repeati (k - 1) (bn_lshift1_mod_n n) b in
     bn_mul_by_pow2 len n b (k - 1);
     assert (bn_v res0 == pow2 (k - 1) * bn_v b % bn_v n);
-    unfold_repeati k (bn_lshift1_mod_n n) b (k - 1);
+    Loops.unfold_repeati k (bn_lshift1_mod_n n) b (k - 1);
     assert (res == bn_lshift1_mod_n n (k - 1) res0);
     bn_lshift1_mod_n_lemma n (k - 1) res0;
     assert (bn_v res == 2 * (pow2 (k - 1) * bn_v b % bn_v n) % bn_v n);
@@ -61,19 +61,19 @@ let rec bn_mul_by_pow2 #t len n b k =
 
 let bn_precomp_r2_mod_n #t #nLen nBits n =
   let c = create nLen (uint #t 0) in
-  let c0 = bn_set_ith_bit c nBits in // c0 == pow2 nBits
+  let c0 = BN.bn_set_ith_bit c nBits in // c0 == pow2 nBits
   // pow2 (2 * bits t * nLen) / pow2 nBits == pow2 (2 * bits t * nLen - nBits)
 
-  repeati (2 * bits t * nLen - nBits) (bn_lshift1_mod_n n) c0
+  Loops.repeati (2 * bits t * nLen - nBits) (bn_lshift1_mod_n n) c0
 
 
 let bn_precomp_r2_mod_n_lemma #t #nLen nBits n =
   let c = create nLen (uint #t 0) in
-  let c0 = bn_set_ith_bit c nBits in
+  let c0 = BN.bn_set_ith_bit c nBits in
   bn_eval_zeroes #t nLen nLen;
-  bn_set_ith_bit_lemma c nBits;
+  BN.bn_set_ith_bit_lemma c nBits;
   assert (bn_v c0 == pow2 nBits);
-  let res = repeati (2 * bits t * nLen - nBits) (bn_lshift1_mod_n n) c0 in
+  let res = Loops.repeati (2 * bits t * nLen - nBits) (bn_lshift1_mod_n n) c0 in
   bn_mul_by_pow2 nLen n c0 (2 * bits t * nLen - nBits);
   assert (bn_v res == pow2 (2 * bits t * nLen - nBits) * pow2 nBits % bn_v n);
   Math.Lemmas.pow2_plus (2 * bits t * nLen - nBits) nBits;
@@ -94,7 +94,7 @@ val bn_mont_reduction_f:
 
 let bn_mont_reduction_f #t #nLen n mu j (c0, acc) =
   let qj = mu *. acc.[j] in
-  let c1, res1 = bn_mul1_lshift_add n qj j acc in
+  let c1, res1 = BN.bn_mul1_lshift_add n qj j acc in
   let c2, r = addcarry c0 c1 res1.[nLen + j] in
   let res = res1.[nLen + j] <- r in
   c2, res
@@ -103,12 +103,12 @@ let bn_mont_reduction_t (#t:limb_t) (#nLen:size_nat{nLen + nLen <= max_size_t}) 
   tuple2 (carry t) (lbignum t (nLen + nLen))
 
 let bn_mont_reduction #t #nLen n mu c =
-  let (c0, c) = repeat_gen nLen bn_mont_reduction_t (bn_mont_reduction_f n mu) (uint #t 0, c) in
-  let res = bn_rshift c nLen in
-  bn_reduce_once n c0 res
+  let (c0, c) = Loops.repeat_gen nLen bn_mont_reduction_t (bn_mont_reduction_f n mu) (uint #t 0, c) in
+  let res = BN.bn_rshift c nLen in
+  BN.bn_reduce_once n c0 res
 
 let bn_to_mont #t #nLen n mu r2 a =
-  let c = bn_mul a r2 in // c = a * r2
+  let c = BN.bn_mul a r2 in // c = a * r2
   bn_mont_reduction n mu c // aM = c % n
 
 let bn_from_mont #t #nLen n mu aM =
@@ -117,11 +117,11 @@ let bn_from_mont #t #nLen n mu aM =
   bn_mont_reduction n mu tmp
 
 let bn_mont_mul #t #nLen n mu aM bM =
-  let c = bn_mul aM bM in // c = aM * bM
+  let c = BN.bn_mul aM bM in // c = aM * bM
   bn_mont_reduction n mu c // resM = c % n
 
 let bn_mont_sqr #t #nLen n mu aM =
-  let c = bn_mul aM aM in // c = aM * aM
+  let c = BN.bn_mul aM aM in // c = aM * aM
   bn_mont_reduction n mu c // resM = c % n
 
 
@@ -182,8 +182,8 @@ let bn_mont_reduction_f_eval_lemma #t #nLen n mu j (c0, res0) =
   let p = pow2 (pbits * (nLen + j)) in
   let resLen = nLen + nLen in
   let qj = mu *. res0.[j] in
-  let c1, res1 = bn_mul1_lshift_add n qj j res0 in
-  bn_mul1_lshift_add_lemma n qj j res0;
+  let c1, res1 = BN.bn_mul1_lshift_add n qj j res0 in
+  BN.bn_mul1_lshift_add_lemma n qj j res0;
   assert (v c1 * p + eval_ resLen res1 (nLen + j) == eval_ resLen res0 (nLen + j) + bn_v n * v qj * pow2 (pbits * j));
 
   let c2, r = addcarry c0 c1 res1.[nLen + j] in
@@ -286,25 +286,25 @@ val bn_mont_reduction_loop_lemma:
   -> j:size_nat{j <= nLen}
   -> res0:lbignum t (nLen + nLen) ->
   Lemma (
-    let (c2, res) = repeat_gen j bn_mont_reduction_t (bn_mont_reduction_f n mu) (uint #t 0, res0) in
-    let resM = repeati j (M.mont_reduction_f (bits t) nLen (bn_v n) (v mu)) (bn_v res0) in
+    let (c2, res) = Loops.repeat_gen j bn_mont_reduction_t (bn_mont_reduction_f n mu) (uint #t 0, res0) in
+    let resM = Loops.repeati j (M.mont_reduction_f (bits t) nLen (bn_v n) (v mu)) (bn_v res0) in
     v c2 * pow2 (bits t * (nLen + j)) + bn_v res == resM)
 
 let rec bn_mont_reduction_loop_lemma #t #nLen n mu j res0 =
   let pbits = bits t in
-  let (c2, res) = repeat_gen j bn_mont_reduction_t (bn_mont_reduction_f n mu) (uint #t 0, res0) in
-  let resM = repeati j (M.mont_reduction_f pbits nLen (bn_v n) (v mu)) (bn_v res0) in
+  let (c2, res) = Loops.repeat_gen j bn_mont_reduction_t (bn_mont_reduction_f n mu) (uint #t 0, res0) in
+  let resM = Loops.repeati j (M.mont_reduction_f pbits nLen (bn_v n) (v mu)) (bn_v res0) in
 
   if j = 0 then begin
-    eq_repeati0 j (M.mont_reduction_f pbits nLen (bn_v n) (v mu)) (bn_v res0);
-    eq_repeat_gen0 j bn_mont_reduction_t (bn_mont_reduction_f n mu) (uint #t 0, res0);
+    Loops.eq_repeati0 j (M.mont_reduction_f pbits nLen (bn_v n) (v mu)) (bn_v res0);
+    Loops.eq_repeat_gen0 j bn_mont_reduction_t (bn_mont_reduction_f n mu) (uint #t 0, res0);
     () end
   else begin
-    let (c1, res1) = repeat_gen (j - 1) bn_mont_reduction_t (bn_mont_reduction_f n mu) (uint #t 0, res0) in
-    let resM1 = repeati (j - 1) (M.mont_reduction_f pbits nLen (bn_v n) (v mu)) (bn_v res0) in
-    unfold_repeat_gen j bn_mont_reduction_t (bn_mont_reduction_f n mu) (uint #t 0, res0) (j - 1);
+    let (c1, res1) = Loops.repeat_gen (j - 1) bn_mont_reduction_t (bn_mont_reduction_f n mu) (uint #t 0, res0) in
+    let resM1 = Loops.repeati (j - 1) (M.mont_reduction_f pbits nLen (bn_v n) (v mu)) (bn_v res0) in
+    Loops.unfold_repeat_gen j bn_mont_reduction_t (bn_mont_reduction_f n mu) (uint #t 0, res0) (j - 1);
     assert ((c2, res) == bn_mont_reduction_f n mu (j - 1) (c1, res1));
-    unfold_repeati j (M.mont_reduction_f pbits nLen (bn_v n) (v mu)) (bn_v res0) (j - 1);
+    Loops.unfold_repeati j (M.mont_reduction_f pbits nLen (bn_v n) (v mu)) (bn_v res0) (j - 1);
     assert (resM == M.mont_reduction_f pbits nLen (bn_v n) (v mu) (j - 1) resM1);
     bn_mont_reduction_loop_lemma n mu (j - 1) res0;
     assert (v c1 * pow2 (pbits * (nLen + j - 1)) + bn_v res1 == resM1);
@@ -315,12 +315,12 @@ let rec bn_mont_reduction_loop_lemma #t #nLen n mu j res0 =
 let bn_mont_reduction_lemma #t #nLen n mu res0 =
   let pbits = bits t in
   let resLen = nLen + nLen in
-  let (c0, res1) = repeat_gen nLen bn_mont_reduction_t (bn_mont_reduction_f n mu) (uint #t 0, res0) in
-  let resM : nat = repeati nLen (M.mont_reduction_f pbits nLen (bn_v n) (v mu)) (bn_v res0) in
+  let (c0, res1) = Loops.repeat_gen nLen bn_mont_reduction_t (bn_mont_reduction_f n mu) (uint #t 0, res0) in
+  let resM : nat = Loops.repeati nLen (M.mont_reduction_f pbits nLen (bn_v n) (v mu)) (bn_v res0) in
   bn_mont_reduction_loop_lemma n mu nLen res0;
   assert (v c0 * pow2 (pbits * resLen) + bn_v res1 == resM);
-  let res2 = bn_rshift res1 nLen in
-  bn_rshift_lemma res1 nLen;
+  let res2 = BN.bn_rshift res1 nLen in
+  BN.bn_rshift_lemma res1 nLen;
   assert (bn_v res2 == bn_v res1 / pow2 (pbits * nLen));
 
   calc (==) {
@@ -339,8 +339,8 @@ let bn_mont_reduction_lemma #t #nLen n mu res0 =
   M.mont_mult_lemma_fits_aux pbits nLen (bn_v n) (v mu) (bn_v res0);
   assert (resM / pow2 (pbits * nLen) < 2 * bn_v n);
 
-  let res3 = bn_reduce_once n c0 res2 in
-  bn_reduce_once_lemma n c0 res2;
+  let res3 = BN.bn_reduce_once n c0 res2 in
+  BN.bn_reduce_once_lemma n c0 res2;
   assert (bn_v res3 == (v c0 * pow2 (pbits * nLen) + bn_v res2) % bn_v n);
 
   let resM1 = resM / pow2 (pbits * nLen) in
@@ -353,8 +353,8 @@ let bn_mont_reduction_lemma #t #nLen n mu res0 =
 
 
 let bn_to_mont_lemma #t #nLen n mu r2 a =
-  let c = bn_mul a r2 in // c = a * r2
-  bn_mul_lemma a r2;
+  let c = BN.bn_mul a r2 in // c = a * r2
+  BN.bn_mul_lemma a r2;
   Math.Lemmas.lemma_mult_lt_sqr (bn_v a) (bn_v r2) (bn_v n);
   assert (bn_v c < bn_v n * bn_v n);
 
@@ -368,6 +368,7 @@ let bn_from_mont_lemma #t #nLen n mu aM =
   let tmp = update_sub tmp 0 nLen aM in
   bn_eval_update_sub nLen aM (nLen + nLen);
   assert (bn_v tmp == bn_v aM);
+  assert (bn_v tmp < bn_v n);
 
   let a = bn_mont_reduction n mu tmp in
   bn_mont_reduction_lemma n mu tmp;
@@ -375,8 +376,8 @@ let bn_from_mont_lemma #t #nLen n mu aM =
 
 
 let bn_mont_mul_lemma #t #nLen n mu aM bM =
-  let c = bn_mul aM bM in
-  bn_mul_lemma aM bM;
+  let c = BN.bn_mul aM bM in
+  BN.bn_mul_lemma aM bM;
   assert (bn_v c == bn_v aM * bn_v bM);
   Math.Lemmas.lemma_mult_lt_sqr (bn_v aM) (bn_v bM) (bn_v n);
   assert (bn_v c < bn_v n * bn_v n);
@@ -384,8 +385,8 @@ let bn_mont_mul_lemma #t #nLen n mu aM bM =
 
 
 let bn_mont_sqr_lemma #t #nLen n mu aM =
-  let c = bn_mul aM aM in
-  bn_mul_lemma aM aM;
+  let c = BN.bn_mul aM aM in
+  BN.bn_mul_lemma aM aM;
   assert (bn_v c == bn_v aM * bn_v aM);
   Math.Lemmas.lemma_mult_lt_sqr (bn_v aM) (bn_v aM) (bn_v n);
   assert (bn_v c < bn_v n * bn_v n);
