code/bignum/Hacl.Spec.Bignum.Montgomery.fsti
@@ -10,6 +10,11 @@ module M = Hacl.Spec.Montgomery.Lemmas
 
 #reset-options "--z3rlimit 50 --fuel 0 --ifuel 0"
 
+let bn_mont_pre (#t:limb_t) (#nLen:size_pos) (n:lbignum t nLen) (mu:limb t) =
+  (1 + (bn_v n % pow2 (bits t)) * v mu) % pow2 (bits t) == 0 /\
+  bn_v n % 2 = 1 /\ 1 < bn_v n
+
+
 ///  Check a modulus for Montgomery arithmetic
 val bn_check_modulus: #t:limb_t -> #nLen:size_pos{2 * bits t * nLen <= max_size_t} -> n:lbignum t nLen ->
   res:limb t{v res == (if (bn_v n % 2 = 1 && 1 < bn_v n) then v (ones t SEC) else v (zeros t SEC))}
@@ -85,9 +90,7 @@ val bn_mont_reduction_lemma:
   -> mu:limb t
   -> c:lbignum t (nLen + nLen) -> Lemma
   (requires
-    (1 + (bn_v n % pow2 (bits t)) * v mu) % pow2 (bits t) == 0 /\
-    bn_v n % 2 = 1 /\ 1 < bn_v n /\
-    bn_v c < bn_v n * bn_v n)
+    bn_mont_pre n mu /\ bn_v c < bn_v n * bn_v n)
   (ensures
     (let res = bn_v (bn_mont_reduction n mu c) in
     res == M.mont_reduction (bits t) nLen (bn_v n) (v mu) (bn_v c) /\
@@ -102,9 +105,8 @@ val bn_to_mont_lemma:
   -> r2:lbignum t nLen
   -> a:lbignum t nLen -> Lemma
   (requires
-    (1 + (bn_v n % pow2 (bits t)) * v mu) % pow2 (bits t) == 0 /\
-    bn_v n % 2 = 1 /\ 1 < bn_v n /\
-    bn_v a < bn_v n /\ bn_v r2 == pow2 (2 * bits t * nLen) % bn_v n)
+    bn_mont_pre n mu /\ bn_v a < bn_v n /\
+    bn_v r2 == pow2 (2 * bits t * nLen) % bn_v n)
   (ensures
    (let aM = bn_v (bn_to_mont n mu r2 a) in
     aM == M.to_mont (bits t) nLen (bn_v n) (v mu) (bn_v a) /\
@@ -118,9 +120,7 @@ val bn_from_mont_lemma:
   -> mu:limb t
   -> aM:lbignum t nLen -> Lemma
   (requires
-    (1 + (bn_v n % pow2 (bits t)) * v mu) % pow2 (bits t) == 0 /\
-    bn_v n % 2 = 1 /\ 1 < bn_v n /\
-    bn_v aM < bn_v n)
+    bn_mont_pre n mu /\ bn_v aM < bn_v n)
   (ensures
    (let a = bn_v (bn_from_mont n mu aM) in
     a == M.from_mont (bits t) nLen (bn_v n) (v mu) (bn_v aM) /\
@@ -135,8 +135,7 @@ val bn_mont_mul_lemma:
   -> aM:lbignum t nLen
   -> bM:lbignum t nLen -> Lemma
   (requires
-    (1 + (bn_v n % pow2 (bits t)) * v mu) % pow2 (bits t) == 0 /\
-    bn_v n % 2 = 1 /\ 1 < bn_v n /\
+    bn_mont_pre n mu /\
     bn_v aM < bn_v n /\ bn_v bM < bn_v n)
   (ensures
     (let res = bn_v (bn_mont_mul n mu aM bM) in
@@ -151,9 +150,7 @@ val bn_mont_sqr_lemma:
   -> mu:limb t
   -> aM:lbignum t nLen -> Lemma
   (requires
-    (1 + (bn_v n % pow2 (bits t)) * v mu) % pow2 (bits t) == 0 /\
-    bn_v n % 2 = 1 /\ 1 < bn_v n /\
-    bn_v aM < bn_v n)
+    bn_mont_pre n mu /\ bn_v aM < bn_v n)
   (ensures
     (let res = bn_v (bn_mont_sqr n mu aM) in
     res == M.mont_mul (bits t) nLen (bn_v n) (v mu) (bn_v aM) (bn_v aM) /\
