code/bignum/Hacl.Spec.Bignum.ExponentiationPrecomp.fst
@@ -1,0 +1,403 @@
+module Hacl.Spec.Bignum.ExponentiationPrecomp
+
+open FStar.Mul
+
+open Lib.IntTypes
+open Lib.Sequence
+
+open Hacl.Spec.Bignum.Definitions
+
+module Loops = Lib.LoopCombinators
+module LSeq = Lib.Sequence
+
+module E = Hacl.Spec.Exponentiation.Lemmas
+module M = Hacl.Spec.Montgomery.Lemmas
+
+module BE = Hacl.Spec.Bignum.Exponentiation
+module BM = Hacl.Spec.Bignum.Montgomery
+module BN = Hacl.Spec.Bignum
+module BI = Hacl.Spec.Bignum.ModInvLimb
+
+#reset-options "--z3rlimit 50 --fuel 0 --ifuel 0"
+
+val bn_mod_exp_mont_pow2:
+    #t:limb_t
+  -> #nLen:size_pos{nLen + nLen <= max_size_t}
+  -> n:lbignum t nLen
+  -> mu:limb t
+  -> aM:lbignum t nLen
+  -> b:size_nat ->
+  lbignum t nLen
+
+let bn_mod_exp_mont_pow2 #t #nLen n mu aM b =
+  Loops.repeat b (BM.bn_mont_sqr n mu) aM
+
+
+val bn_mod_exp_mont_pow2_lemma:
+    #t:limb_t
+  -> #nLen:size_pos{nLen + nLen <= max_size_t}
+  -> n:lbignum t nLen
+  -> mu:limb t
+  -> aM:lbignum t nLen
+  -> b:size_nat -> Lemma
+  (requires
+    BM.bn_mont_pre n mu /\ bn_v aM < bn_v n)
+  (ensures
+   (let r = bn_mod_exp_mont_pow2 #t #nLen n mu aM b in bn_v r < bn_v n /\
+    bn_v r == E.mod_exp_mont_pow2 (bits t) nLen (bn_v n) (v mu) (bn_v aM) b))
+
+let rec bn_mod_exp_mont_pow2_lemma #t #nLen n mu aM b =
+  if b = 0 then begin
+    Loops.eq_repeat0 (BM.bn_mont_sqr n mu) aM;
+    Loops.eq_repeat0 (M.mont_sqr (bits t) nLen (bn_v n) (v mu)) (bn_v aM);
+    BM.bn_mont_sqr_lemma n mu aM end
+  else begin
+    let r1 = bn_mod_exp_mont_pow2 #t #nLen n mu aM (b - 1) in
+    Loops.unfold_repeat b (BM.bn_mont_sqr n mu) aM (b - 1);
+    Loops.unfold_repeat b (M.mont_sqr (bits t) nLen (bn_v n) (v mu)) (bn_v aM) (b - 1);
+    bn_mod_exp_mont_pow2_lemma #t #nLen n mu aM (b - 1);
+    BM.bn_mont_sqr_lemma n mu r1;
+    () end
+
+
+val bn_mod_exp_mont_precomp_table_f:
+    #t:limb_t
+  -> #nLen:size_pos
+  -> n:lbignum t nLen
+  -> mu:limb t
+  -> aM:lbignum t nLen
+  -> table_len:size_nat{1 < table_len /\ table_len * nLen <= max_size_t}
+  -> i:nat{i < table_len - 2}
+  -> table:lbignum t (table_len * nLen) ->
+  lbignum t (table_len * nLen)
+
+let bn_mod_exp_mont_precomp_table_f #t #nLen n mu aM table_len i table =
+  let t1 = sub table ((i + 1) * nLen) nLen in
+  let r = BM.bn_mont_mul n mu t1 aM in
+  update_sub table ((i + 2) * nLen) nLen r
+
+
+val bn_mod_exp_mont_precomp_table:
+    #t:limb_t
+  -> #nLen:size_pos
+  -> n:lbignum t nLen
+  -> mu:limb t
+  -> table_len:size_nat{1 < table_len /\ table_len * nLen <= max_size_t}
+  -> aM:lbignum t nLen
+  -> oneM:lbignum t nLen ->
+  lbignum t (table_len * nLen)
+
+let bn_mod_exp_mont_precomp_table #t #nLen n mu table_len aM oneM =
+  let table = create (table_len * nLen) (uint #t 0) in
+  let table = update_sub table 0 nLen oneM in
+  let table = update_sub table nLen nLen aM in
+
+  Loops.repeati (table_len - 2) (bn_mod_exp_mont_precomp_table_f n mu aM table_len) table
+
+
+val bn_mod_exp_mont_precomp_table_loop_lemma:
+    #t:limb_t
+  -> #nLen:size_pos
+  -> n:lbignum t nLen
+  -> mu:limb t
+  -> table_len:size_nat{1 < table_len /\ table_len * nLen <= max_size_t}
+  -> aM:lbignum t nLen
+  -> t01:lbignum t (table_len * nLen)
+  -> t02:lseq nat table_len
+  -> j:nat{j <= table_len - 2} -> Lemma
+  (requires
+    BM.bn_mont_pre n mu /\ bn_v aM < bn_v n /\
+    index t02 0 == bn_v (sub t01 0 nLen) /\
+    index t02 1 == bn_v (sub t01 nLen nLen))
+  (ensures
+   (let t3 : lbignum t (table_len * nLen) = Loops.repeati j (bn_mod_exp_mont_precomp_table_f n mu aM table_len) t01 in
+    let t4 : lseq nat table_len = Loops.repeati j
+      (E.mod_exp_mont_precomp_table_f (bits t) nLen (bn_v n) (v mu) (bn_v aM) table_len) t02 in
+    (forall (i:nat{i < j + 2}).
+     (Math.Lemmas.lemma_mult_le_right nLen (i + 1) (table_len);
+      assert (i * nLen + nLen <= table_len * nLen);
+      let bi = sub t3 (i * nLen) nLen in bn_v bi == index t4 i))))
+
+let bn_mod_exp_mont_precomp_table_loop_lemma #t #nLen n mu table_len aM t01 t02 j =
+  admit()
+
+
+val bn_mod_exp_mont_precomp_table_lemma:
+    #t:limb_t
+  -> #nLen:size_pos
+  -> n:lbignum t nLen
+  -> mu:limb t
+  -> table_len:size_nat{1 < table_len /\ table_len * nLen <= max_size_t}
+  -> aM:lbignum t nLen
+  -> oneM:lbignum t nLen -> Lemma
+  (requires
+    BM.bn_mont_pre n mu /\ bn_v aM < bn_v n /\
+    bn_v oneM == M.to_mont (bits t) nLen (bn_v n) (v mu) 1)
+  (ensures
+   (let t1 : lbignum t (table_len * nLen) = bn_mod_exp_mont_precomp_table n mu table_len aM oneM in
+    let t2 : lseq nat table_len = E.mod_exp_mont_precomp_table (bits t) nLen (bn_v n) (v mu) table_len (bn_v aM) in
+    (forall (i:nat{i < table_len}).
+     (Math.Lemmas.lemma_mult_le_right nLen (i + 1) (table_len);
+      assert (i * nLen + nLen <= table_len * nLen);
+      let bi = sub t1 (i * nLen) nLen in bn_v bi == index t2 i))))
+
+let bn_mod_exp_mont_precomp_table_lemma #t #nLen n mu table_len aM oneM =
+  let t01 = create (table_len * nLen) (uint #t 0) in
+  let t01' = update_sub t01 0 nLen oneM in
+  let t01 = update_sub t01' nLen nLen aM in
+
+  let t02 = create table_len 0 in
+  let t02' = t02.[0] <- bn_v oneM in
+  let t02 = t02'.[1] <- bn_v aM in
+  LSeq.eq_intro (sub t01 0 nLen) (sub t01' 0 nLen);
+  assert (index t02 0 == bn_v (sub t01 0 nLen));
+  assert (index t02 1 == bn_v (sub t01 nLen nLen));
+  bn_mod_exp_mont_precomp_table_loop_lemma #t #nLen n mu table_len aM t01 t02 (table_len - 2)
+
+
+val bn_mod_exp_mont_precomp_f:
+    #t:limb_t
+  -> #nLen:size_pos
+  -> n:lbignum t nLen
+  -> mu:limb t
+  -> bBits:size_pos
+  -> bLen:size_nat{bLen == blocks bBits (bits t)}
+  -> b:lbignum t bLen
+  -> l:size_nat{l <= bits t}
+  -> table_len:size_nat{1 < table_len /\ table_len * nLen <= max_size_t /\ table_len == pow2 l}
+  -> table:lbignum t (table_len * nLen)
+  -> i:nat{l * (i + 1) <= bBits}
+  -> accM:lbignum t nLen ->
+  lbignum t nLen
+
+let bn_mod_exp_mont_precomp_f #t #nLen n mu bBits bLen b l table_len table i accM =
+  let bits_l = BN.bn_get_bits b (bBits - l * i - l) l in
+  BN.bn_get_bits_lemma b (bBits - l * i - l) l;
+  assert (v bits_l < table_len);
+  let acc_pow2l = bn_mod_exp_mont_pow2 n mu accM l in
+  Math.Lemmas.lemma_mult_le_right nLen (v bits_l + 1) table_len;
+  let a_powbits_l = sub table (v bits_l * nLen) nLen in
+  BM.bn_mont_mul n mu acc_pow2l a_powbits_l
+
+
+#set-options "--z3rlimit 150"
+val bn_mod_exp_mont_precomp_f_lemma:
+    #t:limb_t
+  -> #nLen:size_pos
+  -> n:lbignum t nLen
+  -> mu:limb t
+  -> bBits:size_pos
+  -> bLen:size_nat{bLen == blocks bBits (bits t)}
+  -> b:lbignum t bLen
+  -> l:size_nat{l <= bits t}
+  -> table_len:size_nat{1 < table_len /\ table_len * nLen <= max_size_t /\ table_len == pow2 l}
+  -> t1:lbignum t (table_len * nLen)
+  -> t2:lseq nat table_len
+  -> oneM:lbignum t nLen
+  -> aM:lbignum t nLen
+  -> i:nat{l * (i + 1) <= bBits}
+  -> accM:lbignum t nLen -> Lemma
+  (requires
+    BM.bn_mont_pre n mu /\ bn_v aM < bn_v n /\
+    bn_v accM < bn_v n /\ bn_v b < pow2 bBits /\
+    bn_v oneM == M.to_mont (bits t) nLen (bn_v n) (v mu) 1 /\
+    t1 == bn_mod_exp_mont_precomp_table n mu table_len aM oneM /\
+    t2 == E.mod_exp_mont_precomp_table (bits t) nLen (bn_v n) (v mu) table_len (bn_v aM))
+  (ensures
+   (let r1 = bn_mod_exp_mont_precomp_f n mu bBits bLen b l table_len t1 i accM in
+    let r2 = E.mod_exp_mont_precomp_f_ll (bits t) nLen (bn_v n) (v mu) bBits (bn_v b) l table_len t2 i (bn_v accM) in
+    bn_v r1 == r2))
+
+let bn_mod_exp_mont_precomp_f_lemma #t #nLen n mu bBits bLen b l table_len t1 t2 oneM aM i accM =
+  let bits_l = BN.bn_get_bits b (bBits - l * i - l) l in
+  BN.bn_get_bits_lemma b (bBits - l * i - l) l;
+  assert (v bits_l == bn_v b / pow2 (bBits - l * i - l) % table_len);
+  assert (v bits_l < table_len);
+  let acc_pow2l = bn_mod_exp_mont_pow2 n mu accM l in
+  bn_mod_exp_mont_pow2_lemma n mu accM l;
+  bn_eval_bound n nLen;
+  M.mont_preconditions (bits t) nLen (bn_v n) (v mu);
+  E.mod_exp_mont_pow2_lemma (bits t) nLen (bn_v n) (v mu) (bn_v accM) l;
+  assert (bn_v acc_pow2l < bn_v n);
+
+  Math.Lemmas.lemma_mult_le_right nLen (v bits_l + 1) table_len;
+  let a_powbits_l = sub t1 (v bits_l * nLen) nLen in
+  bn_mod_exp_mont_precomp_table_lemma n mu table_len aM oneM;
+  E.mod_exp_mont_precomp_table_lemma (bits t) nLen (bn_v n) (v mu) table_len (bn_v aM) (v bits_l);
+  assert (bn_v a_powbits_l < bn_v n);
+
+  let res = BM.bn_mont_mul n mu acc_pow2l a_powbits_l in
+  BM.bn_mont_mul_lemma n mu acc_pow2l a_powbits_l
+
+
+// val bn_mod_exp_mont_precomp_loop_lemma:
+//     #t:limb_t
+//   -> #nLen:size_pos
+//   -> n:lbignum t nLen
+//   -> mu:limb t
+//   -> bBits:size_pos
+//   -> bLen:size_nat{bLen == blocks bBits (bits t)}
+//   -> b:lbignum t bLen
+//   -> l:size_pos{l <= bits t}
+//   -> table_len:size_nat{1 < table_len /\ table_len * nLen <= max_size_t /\ table_len == pow2 l}
+//   -> t1:lbignum t (table_len * nLen)
+//   -> t2:lseq nat table_len
+//   -> oneM:lbignum t nLen
+//   -> aM:lbignum t nLen
+//   -> j:nat{j <= bBits / l}
+//   -> accM:lbignum t nLen -> Lemma
+//   (requires
+//     BM.bn_mont_pre n mu /\ E.mont_pre (bits t) nLen (bn_v n) (v mu) /\
+//     bn_v aM < bn_v n /\ bn_v accM < bn_v n /\ bn_v b < pow2 bBits /\
+//     bn_v oneM == M.to_mont (bits t) nLen (bn_v n) (v mu) 1 /\
+//     t1 == bn_mod_exp_mont_precomp_table n mu table_len aM oneM /\
+//     t2 == E.mod_exp_mont_precomp_table (bits t) nLen (bn_v n) (v mu) table_len (bn_v aM))
+//   (ensures
+//    (Math.Lemmas.multiply_fractions bBits l;
+//     Math.Lemmas.lemma_mult_le_left l j (bBits / l);
+//     assert (l * (bBits / l) <= bBits);
+//     let r1 : lbignum t nLen = Loops.repeati j (bn_mod_exp_mont_precomp_f n mu bBits bLen b l table_len t1) accM in
+//     let r2 = Loops.repeati j (E.mod_exp_mont_precomp_f_ll (bits t) nLen (bn_v n) (v mu) bBits (bn_v b) l table_len t2) (bn_v accM) in
+//     bn_v r1 == r2))
+
+// let rec bn_mod_exp_mont_precomp_loop_lemma #t #nLen n mu bBits bLen b l table_len t1 t2 oneM aM j accM =
+//   Math.Lemmas.multiply_fractions bBits l;
+//   Math.Lemmas.lemma_mult_le_left l j (bBits / l);
+//   assert (l * (bBits / l) <= bBits);
+//   let r1 : lbignum t nLen = Loops.repeati j (bn_mod_exp_mont_precomp_f n mu bBits bLen b l table_len t1) accM in
+//   let r2 = Loops.repeati j (E.mod_exp_mont_precomp_f_ll (bits t) nLen (bn_v n) (v mu) bBits (bn_v b) l table_len t2) (bn_v accM) in
+
+//   if j = 0 then begin
+//     Loops.eq_repeati0 j (bn_mod_exp_mont_precomp_f n mu bBits bLen b l table_len t1) accM;
+//     Loops.eq_repeati0 j (E.mod_exp_mont_precomp_f_ll (bits t) nLen (bn_v n) (v mu) bBits (bn_v b) l table_len t2) (bn_v accM) end
+//   else begin
+//     //let r3 = Loops.repeati (j - 1) (bn_mod_exp_mont_precomp_f n mu bBits bLen b l table_len t1) accM in
+//     //Loops.unfold_repeati j (bn_mod_exp_mont_precomp_f n mu bBits bLen b l table_len t1) accM (j - 1);
+//     //Loops.unfold_repeati j (E.mod_exp_mont_precomp_f_ll (bits t) nLen (bn_v n) (v mu) bBits (bn_v b) l table_len t2) (bn_v accM) (j - 1);
+//     //bn_mod_exp_mont_precomp_loop_lemma n mu bBits bLen b l table_len t1 t2 oneM aM (j - 1) accM;
+//     //bn_mod_exp_mont_precomp_f_lemma n mu bBits bLen b l table_len t1 t2 oneM aM (j - 1) r3;
+//     admit() end
+
+
+
+val bn_mod_exp_mont_precomp_rem:
+    #t:limb_t
+  -> #nLen:size_pos
+  -> n:lbignum t nLen
+  -> mu:limb t
+  -> bBits:size_pos
+  -> bLen:size_nat{bLen == blocks bBits (bits t)}
+  -> b:lbignum t bLen
+  -> l:size_pos{l <= bits t}
+  -> table_len:size_nat{1 < table_len /\ table_len * nLen <= max_size_t /\ table_len == pow2 l}
+  -> table:lbignum t (table_len * nLen)
+  -> accM:lbignum t nLen ->
+  lbignum t nLen
+
+let bn_mod_exp_mont_precomp_rem #t #nLen n mu bBits bLen b l table_len table accM =
+  let c = bBits % l in
+  let bits_c = BN.bn_get_bits b 0 c in
+  BN.bn_get_bits_lemma b 0 c;
+  let acc_pow2c = bn_mod_exp_mont_pow2 n mu accM c in
+  Math.Lemmas.pow2_lt_compat l c;
+  Math.Lemmas.lemma_mult_le_right nLen (v bits_c + 1) table_len;
+  let a_powbits_c = sub table (v bits_c * nLen) nLen in
+  BM.bn_mont_mul n mu acc_pow2c a_powbits_c
+
+
+val bn_mod_exp_mont_precomp_rem_lemma:
+    #t:limb_t
+  -> #nLen:size_pos
+  -> n:lbignum t nLen
+  -> mu:limb t
+  -> bBits:size_pos
+  -> bLen:size_nat{bLen == blocks bBits (bits t)}
+  -> b:lbignum t bLen
+  -> l:size_pos{l <= bits t}
+  -> table_len:size_nat{1 < table_len /\ table_len * nLen <= max_size_t /\ table_len == pow2 l}
+  -> t1:lbignum t (table_len * nLen)
+  -> t2:lseq nat table_len
+  -> oneM:lbignum t nLen
+  -> aM:lbignum t nLen
+  -> accM:lbignum t nLen -> Lemma
+  (requires
+    BM.bn_mont_pre n mu /\ bn_v aM < bn_v n /\
+    bn_v accM < bn_v n /\ bn_v b < pow2 bBits /\
+    bn_v oneM == M.to_mont (bits t) nLen (bn_v n) (v mu) 1 /\
+    t1 == bn_mod_exp_mont_precomp_table n mu table_len aM oneM /\
+    t2 == E.mod_exp_mont_precomp_table (bits t) nLen (bn_v n) (v mu) table_len (bn_v aM))
+  (ensures
+   (let r1 = bn_mod_exp_mont_precomp_rem n mu bBits bLen b l table_len t1 accM in
+    let r2 = E.mod_exp_mont_precomp_rem_ll (bits t) nLen (bn_v n) (v mu) bBits (bn_v b) l table_len t2 (bn_v accM) in
+    bn_v r1 == r2))
+
+
+let bn_mod_exp_mont_precomp_rem_lemma #t #nLen n mu bBits bLen b l table_len t1 t2 oneM aM accM =
+  let c = bBits % l in
+  let bits_c = BN.bn_get_bits b 0 c in
+  BN.bn_get_bits_lemma b 0 c;
+  assert_norm (pow2 0 = 1);
+  assert (v bits_c == bn_v b % pow2 c);
+  Math.Lemmas.pow2_lt_compat l c;
+  assert (v bits_c < table_len);
+
+  let acc_pow2c = bn_mod_exp_mont_pow2 n mu accM c in
+  bn_mod_exp_mont_pow2_lemma n mu accM c;
+  bn_eval_bound n nLen;
+  M.mont_preconditions (bits t) nLen (bn_v n) (v mu);
+  E.mod_exp_mont_pow2_lemma (bits t) nLen (bn_v n) (v mu) (bn_v accM) c;
+  assert (bn_v acc_pow2c < bn_v n);
+
+  Math.Lemmas.lemma_mult_le_right nLen (v bits_c + 1) table_len;
+  let a_powbits_c = sub t1 (v bits_c * nLen) nLen in
+  bn_mod_exp_mont_precomp_table_lemma n mu table_len aM oneM;
+  E.mod_exp_mont_precomp_table_lemma (bits t) nLen (bn_v n) (v mu) table_len (bn_v aM) (v bits_c);
+  assert (bn_v a_powbits_c < bn_v n);
+
+  let res = BM.bn_mont_mul n mu acc_pow2c a_powbits_c in
+  BM.bn_mont_mul_lemma n mu acc_pow2c a_powbits_c
+
+
+val bn_mod_exp_fw_precomp_table:
+    #t:limb_t
+  -> #nLen:size_pos{nLen + nLen <= max_size_t}
+  -> n:lbignum t nLen
+  -> mu:limb t
+  -> aM:lbignum t nLen
+  -> bBits:size_pos
+  -> b:lbignum t (blocks bBits (bits t))
+  -> l:size_pos{l <= bits t /\ pow2 l * nLen <= max_size_t}
+  -> r2:lbignum t nLen ->
+  lbignum t nLen
+
+let bn_mod_exp_fw_precomp_table #t #nLen n mu aM bBits b l r2 =
+  let bLen = blocks bBits (bits t) in
+  let one = BN.bn_from_uint nLen (uint #t 1) in
+  let oneM = BM.bn_to_mont n mu r2 one in
+
+  let table_len = pow2 l in
+  Math.Lemmas.pow2_le_compat l 1;
+  let table = bn_mod_exp_mont_precomp_table n mu table_len aM oneM in
+  let accM  = Loops.repeati (bBits / l) (bn_mod_exp_mont_precomp_f #t #nLen n mu bBits bLen b l table_len table) oneM in
+  let res = bn_mod_exp_mont_precomp_rem #t #nLen n mu bBits bLen b l table_len table accM in
+  res
+
+
+let bn_mod_exp_fw_precompr2 #t nLen n a bBits b l r2 =
+  let mu = BI.mod_inv_limb n.[0] in
+  let aM = BM.bn_to_mont n mu r2 a in
+  let resM = bn_mod_exp_fw_precomp_table #t #nLen n mu aM bBits b l r2 in
+  BM.bn_from_mont n mu resM
+
+
+let bn_mod_exp_fw_precompr2_lemma #t nLen n a bBits b l r2 = admit()
+
+
+let bn_mod_exp_fw #t nLen nBits n a bBits b l =
+  let r2 = BM.bn_precomp_r2_mod_n nBits n in
+  bn_mod_exp_fw_precompr2 #t nLen n a bBits b l r2
+
+let bn_mod_exp_fw_lemma #t nLen nBits n a bBits b l =
+  let r2 = BM.bn_precomp_r2_mod_n nBits n in
+  BM.bn_precomp_r2_mod_n_lemma nBits n;
+  bn_mod_exp_fw_precompr2_lemma #t nLen n a bBits b l r2
