code/bignum/Hacl.Spec.Bignum.ExponentiationPrecomp.fsti
@@ -1,0 +1,66 @@
+module Hacl.Spec.Bignum.ExponentiationPrecomp
+
+open FStar.Mul
+
+open Lib.IntTypes
+open Lib.Sequence
+
+open Hacl.Spec.Bignum.Definitions
+
+module BM = Hacl.Spec.Bignum.Montgomery
+module BE = Hacl.Spec.Bignum.Exponentiation
+
+#reset-options "--z3rlimit 50 --fuel 0 --ifuel 0"
+
+
+val bn_mod_exp_fw_precompr2:
+    #t:limb_t
+  -> nLen:size_pos{2 * bits t * nLen <= max_size_t}
+  -> n:lbignum t nLen
+  -> a:lbignum t nLen
+  -> bBits:size_pos
+  -> b:lbignum t (blocks bBits (bits t))
+  -> l:size_pos{l <= bits t /\ pow2 l * nLen <= max_size_t}
+  -> r2:lbignum t nLen ->
+  lbignum t nLen
+
+
+val bn_mod_exp_fw_precompr2_lemma:
+    #t:limb_t
+  -> nLen:size_pos{2 * bits t * nLen <= max_size_t}
+  -> n:lbignum t nLen
+  -> a:lbignum t nLen
+  -> bBits:size_pos
+  -> b:lbignum t (blocks bBits (bits t))
+  -> l:size_pos{l <= bits t /\ pow2 l * nLen <= max_size_t}
+  -> r2:lbignum t nLen -> Lemma
+  (requires
+    BE.bn_mod_exp_pre n a bBits b /\
+    bn_v r2 == pow2 (2 * bits t * nLen) % bn_v n)
+  (ensures
+    BE.bn_mod_exp_post n a bBits b (bn_mod_exp_fw_precompr2 nLen n a bBits b l r2))
+
+
+val bn_mod_exp_fw:
+    #t:limb_t
+  -> nLen:size_pos{2 * bits t * nLen <= max_size_t}
+  -> nBits:size_nat{nBits / bits t < nLen}
+  -> n:lbignum t nLen
+  -> a:lbignum t nLen
+  -> bBits:size_pos
+  -> b:lbignum t (blocks bBits (bits t))
+  -> l:size_pos{l <= bits t /\ pow2 l * nLen <= max_size_t} ->
+  lbignum t nLen
+
+
+val bn_mod_exp_fw_lemma:
+    #t:limb_t
+  -> nLen:size_pos{2 * bits t * nLen <= max_size_t}
+  -> nBits:size_nat{nBits / bits t < nLen}
+  -> n:lbignum t nLen
+  -> a:lbignum t nLen
+  -> bBits:size_pos
+  -> b:lbignum t (blocks bBits (bits t))
+  -> l:size_pos{l <= bits t /\ pow2 l * nLen <= max_size_t} -> Lemma
+  (requires BE.bn_mod_exp_pre n a bBits b /\ pow2 nBits < bn_v n)
+  (ensures  BE.bn_mod_exp_post n a bBits b (bn_mod_exp_fw nLen nBits n a bBits b l))
